finish bvAshr

src/BitBlastingSimple.v
@@ -3783,18 +3783,746 @@ Qed .
 
 
 
-(* ===== bit_blast_sra ===== *)
+(* ===== bit_blast_ashr ===== *)
 
-Definition bit_blast_sra_int1 w (g : generator) (ls: (w.+1).-tuple literal) : generator * cnf * (w.+1).-tuple literal :=
-  (g, [], joinmsb (msb_nonnil ls, droplsb ls)).
+Definition bit_blast_ashr_int1 w (g : generator) (ls: (w.+1).-tuple literal) : generator * cnf * (w.+1).-tuple literal :=
+  (g, [], joinmsb (last lit_ff ls, droplsb ls)) .
 
-Fixpoint bit_blast_sra_int w (g : generator) (ls : (w.+1).-tuple literal) (n : nat) : generator * cnf * (w.+1).-tuple literal :=
+Fixpoint bit_blast_ashr_int w (g : generator) (ls : (w.+1).-tuple literal) (n : nat) : generator * cnf * (w.+1).-tuple literal :=
   match n with
   | O => (g, [], ls)
-  | S m => let '(g_m, cs_m, ls_m) := bit_blast_sra_int g ls m in
-           let '(g1, cs1, ls1) := bit_blast_sra_int1 g_m ls_m in
-           (g1, cs_m++cs1, ls1)
-  end.
+  | S m => let '(g_m, cs_m, ls_m) := bit_blast_ashr_int g ls m in
+           let '(g', cs1, ls') := bit_blast_ashr_int1 g_m ls_m in
+           (g', cs_m++cs1, ls')
+  end .
+
+Definition mk_env_ashr_int1 w (E : env) (g : generator) (ls : (w.+1).-tuple literal) : env * generator * cnf * (w.+1).-tuple literal :=
+  (E, g, [], joinmsb (last lit_ff ls, droplsb ls)) .
+
+Fixpoint mk_env_ashr_int w (E : env) (g : generator) (ls : (w.+1).-tuple literal) (n : nat) : env * generator * cnf * (w.+1).-tuple literal :=
+  match n with
+  | O => (E, g, [], ls)
+  | S m => let: (E_m, g_m, cs_m, ls_m) := mk_env_ashr_int E g ls m in
+           let: (E', g', cs, ls') := mk_env_ashr_int1 E_m g_m ls_m in
+           (E', g', cs_m ++ cs, ls')
+  end .
+
+Lemma bit_blast_ashr_int1_correct :
+  forall w g (bs : BITS (w.+1)) E ls g' cs lrs,
+    bit_blast_ashr_int1 g ls = (g', cs, lrs) ->
+    enc_bits E ls bs ->
+    interp_cnf E (add_prelude cs) ->
+    enc_bits E lrs (sarB bs).
+Proof.
+  move => w g bs E ls g' cs lrs .
+  rewrite /bit_blast_ashr_int1 /sarB .
+  case => _ <- <- Henc _ .
+  rewrite enc_bits_joinmsb .
+  apply /andP; split ; last by apply : enc_bits_droplsb .
+  rewrite /msb .
+  by apply enc_bits_last .
+Qed .
+
+Lemma bit_blast_ashr_int_correct :
+  forall w g (bs : BITS (w.+1)) n E ls g' cs lrs,
+    bit_blast_ashr_int g ls n = (g', cs, lrs) ->
+    enc_bits E ls bs ->
+    interp_cnf E (add_prelude cs) ->
+    enc_bits E lrs (sarBn bs n).
+Proof.
+  move => w g bs .
+  elim .
+  - move => E ls g' cs lrs .
+    case => _ _ <- Hlsbs _ .
+    by rewrite /sarBn /iter .
+  - move => n IH E ls g' cs lrs .
+    rewrite /bit_blast_ashr_int (lock bit_blast_ashr_int1)
+            (lock interp_cnf) /=  -!lock -/bit_blast_ashr_int .
+    move Hm : (bit_blast_ashr_int g ls n) => [[g_m cs_m] ls_m] .
+    move H1 : (bit_blast_ashr_int1 g_m ls_m) => [[g1 cs1] ls1] .
+    case => Hog Hcs Holrs Henc_ibs Hcnf. rewrite <- Holrs.
+    rewrite -Hcs add_prelude_append in Hcnf. move/andP: Hcnf => [Hcnf_m Hcnf1].
+    apply: (bit_blast_ashr_int1_correct H1 _ Hcnf1).
+    exact: (IH E _ _ _ _ Hm Henc_ibs Hcnf_m).
+Qed .    
+
+Fixpoint bit_blast_ashr_rec w wn (g : generator) : (w.+1).-tuple literal -> wn.-tuple literal -> nat -> generator * cnf * (w.+1).-tuple literal :=
+  if wn is _.+1 then
+    fun ls ns i =>
+      let (ns_tl, ns_hd) := eta_expand (splitlsb ns) in
+      let '(g_tl, cs_tl, ls_tl) := bit_blast_ashr_rec g ls ns_tl (2 * i) in
+      let '(g_hd, cs_hd, ls_hd) := bit_blast_ashr_int g_tl ls_tl i in
+      if ns_hd == lit_tt then
+        (g_hd, cs_tl++cs_hd, ls_hd)
+      else if ns_hd == lit_ff then
+             (g_tl, cs_tl, ls_tl)
+           else
+             let '(g_ite, cs_ite, ls_ite) := bit_blast_ite g_hd ns_hd ls_hd ls_tl in
+             (g_ite, cs_tl++cs_hd++cs_ite, ls_ite)
+  else
+    fun ls _ _ =>
+      (g, [], ls).
+
+Definition bit_blast_ashr w (g : generator) (ls ns : (w.+1).-tuple literal) : generator * cnf * (w.+1).-tuple literal :=
+  bit_blast_ashr_rec g ls ns 1.
+
+Fixpoint mk_env_ashr_rec w wn (E : env) (g : generator) : (w.+1).-tuple literal -> wn.-tuple literal -> nat -> env * generator * cnf * (w.+1).-tuple literal :=
+  if wn is _.+1 then
+    fun ls ns i =>
+      let (ns_tl, ns_hd) := eta_expand (splitlsb ns) in
+      let '(E_tl, g_tl, cs_tl, ls_tl) := mk_env_ashr_rec E g ls ns_tl (2 * i) in
+      let '(E_hd, g_hd, cs_hd, ls_hd) := mk_env_ashr_int E_tl g_tl ls_tl i in
+      if ns_hd == lit_tt then
+        (E_hd, g_hd, cs_tl++cs_hd, ls_hd)
+      else if ns_hd == lit_ff then
+             (E_tl, g_tl, cs_tl, ls_tl)
+           else
+             let '(E_ite, g_ite, cs_ite, ls_ite) := mk_env_ite E_hd g_hd ns_hd ls_hd ls_tl in
+             (E_ite, g_ite, cs_tl++cs_hd++cs_ite, ls_ite)
+  else
+    fun ls _ _ =>
+      (E, g, [], ls).
+
+Definition mk_env_ashr w (E : env) (g : generator) (ls ns : (w.+1).-tuple literal) : env * generator * cnf * (w.+1).-tuple literal :=
+  mk_env_ashr_rec E g ls ns 1.
+
+Lemma bit_blast_ashr_rec_correct :
+  forall w wn g (bs : BITS (w.+1)) (ns: BITS wn) i E ls (lns : wn.-tuple literal) g' cs lrs,
+    bit_blast_ashr_rec g ls lns i = (g', cs, lrs) ->
+    enc_bits E ls bs ->
+    enc_bits E lns ns ->
+    interp_cnf E (add_prelude cs) ->
+    enc_bits E lrs (sarBn bs (toNat ns * i)).
+Proof.
+  move => w  .
+  elim .
+  - move => g bs ns i E ls lns g' cs lrs .
+    case => _ <- <- Hlsbs _ _ .
+    by rewrite tuple0 /= .
+  - move => n IH g bs /tupleP [ns_hd ns_tl] i E ls
+              /tupleP [lns_hd lns_tl] g' cs lrs .
+    case Htl : (bit_blast_ashr_rec g ls lns_tl (2 * i))
+    => [[g_tl cs_tl] ls_tl] .
+    case Hhd : (bit_blast_ashr_int g_tl ls_tl i)
+    => [[g_hd cs_hd] ls_hd] .
+    rewrite /bit_blast_ashr_rec -/bit_blast_ashr_rec
+            (lock bit_blast_ite) (lock add_prelude)
+            /= !beheadCons !theadCons Htl Hhd -!lock .
+    case Htt : (lns_hd == lit_tt) .
+    + move /eqP : Htt => Htt . rewrite Htt .
+      case => _ <- <- Hlsbs /andP [Hnshd Hnstl] .
+      rewrite add_prelude_append .
+      case /andP => [Hcstl Hcshd] .
+      rewrite (add_prelude_enc_bit_true _ Hcstl) in Hnshd .
+      rewrite Hnshd .
+      move : (IH _ _ _ _ _ _ _ _ _ _ Htl Hlsbs Hnstl Hcstl)
+      => Hshrlstl .
+      move :(bit_blast_ashr_int_correct Hhd Hshrlstl Hcshd) => Hshrlshd .
+      rewrite -sarBn_add in Hshrlshd .
+      rewrite toNat_joinlsb /= .
+      rewrite -muln2 .
+      by replace ((1 + toNat ns_tl * 2) * i) with (toNat ns_tl * (2 * i) + i) by ring .
+      case Hff : (lns_hd == lit_ff) .
+      * move /eqP : Hff => Hff; rewrite Hff .
+        case => _ <- <- Hlsbs /andP [Hnshd Hnstl] Hcstl .
+        rewrite (add_prelude_enc_bit_is_false _ Hcstl) in Hnshd .
+        rewrite (eqP Hnshd) {Hnshd} .
+        move : (IH _ _ _ _ _ _ _ _ _ _ Htl Hlsbs Hnstl Hcstl) .
+        rewrite toNat_joinlsb /= -muln2 .
+        replace ((0 + toNat ns_tl * 2) * i) with (toNat ns_tl * (2 * i)) by ring .
+        done .
+      * case Hite : (bit_blast_ite g_hd lns_hd ls_hd ls_tl)
+        => {Htt Hff} [[g_ite cs_ite] ls_ite] .
+        case => _ <- <- Hlsbs /andP [Hnshd Hnstl] .
+        rewrite !add_prelude_append; case /andP => [Hcstl Hcshdite] .
+        case : Hcshdite => /andP [Hcshd Hcsite] .
+        move : (IH _ _ _ _ _ _ _ _ _ _ Htl Hlsbs Hnstl Hcstl) => Hlstl .
+        move : (bit_blast_ashr_int_correct Hhd Hlstl Hcshd) => Hlshd .
+        rewrite -sarBn_add in Hlshd .
+        rewrite toNat_joinlsb /= -mul2n .
+        apply (bit_blast_ite_correct Hite Hnshd Hlshd Hlstl Hcsite) .
+        case ns_hd; rewrite /= .
+        {
+          by replace ((1 + 2 * toNat ns_tl) * i) with
+              (toNat ns_tl * (2 * i) + i) by ring .
+        }
+        {
+          by replace ((0 + 2 * toNat ns_tl) * i) with
+              (toNat ns_tl * (2 * i)) by ring .
+        }
+Qed .
+
+Corollary bit_blast_ashr_correct :
+  forall w g (bs : BITS w.+1) (ns : BITS w.+1) E ls lns g' cs lrs,
+    bit_blast_ashr g ls lns = (g', cs, lrs) ->
+    enc_bits E ls bs ->
+    enc_bits E lns ns ->
+    interp_cnf E (add_prelude cs) ->
+    enc_bits E lrs (sarBn bs (toNat ns)).
+Proof.
+  move=> w g bs ns E ls lns g' cs lrs Hshl Henc_bs Henc_ns Hcnf.
+  rewrite -(muln1 (toNat ns)).
+  exact: (bit_blast_ashr_rec_correct Hshl Henc_bs Henc_ns Hcnf).
+Qed.
+
+Lemma mk_env_ashr_int1_is_bit_blast_ashr_int1 :
+  forall w E g (ls: (w.+1).-tuple literal) E' g' cs lrs,
+    mk_env_ashr_int1 E g ls = (E', g', cs, lrs) ->
+    bit_blast_ashr_int1 g ls = (g', cs, lrs).
+Proof.
+  rewrite /mk_env_ashr_int1 /bit_blast_ashr_int1 .
+  case .
+  - move => E g ls E' g' cs lrs; case => _ <- <- <-; trivial .
+  - move => n E g ls E' g' cs lrs; case => _ <- <- <-; trivial .
+Qed .
+
+Lemma mk_env_ashr_int_is_bit_blast_ashr_int :
+  forall w E g (ls: (w.+1).-tuple literal) i E' g' cs lrs,
+    mk_env_ashr_int E g ls i = (E', g', cs, lrs) ->
+    bit_blast_ashr_int g ls i = (g', cs, lrs).
+Proof.
+  move => w E g ls /= .
+  elim .
+  - move => E' g' cs lrs .
+    by case => _ <- <- <- /= .
+  - move => n IH E' g' cs lrs /= .
+    case Henvn : (mk_env_ashr_int E g ls n) => [[[En gn] csn] lrsn] .
+    case Henv1 : (mk_env_ashr_int1 En gn lrsn) => [[[E1 g1] cs1] ls1] .
+    case => _ <- <- <- .
+    by rewrite (IH _ _ _ _ Henvn) .
+Qed .
+
+Lemma mk_env_ashr_rec_is_bit_blast_ashr_rec :
+  forall w wn E g (ls : (w.+1).-tuple literal) (ns : wn.-tuple literal)
+         i E' g' cs lrs,
+    mk_env_ashr_rec E g ls ns i= (E', g', cs, lrs) ->
+    bit_blast_ashr_rec g ls ns i = (g', cs, lrs).
+Proof .
+  move => w . elim .
+  - move => E g ls ns i E' g' cs lrs .
+    rewrite /mk_env_ashr_rec /bit_blast_ashr_rec /= .
+    by case => _ <- <- <- .
+  - move => n IH E g ls . case/tupleP => [ns_hd ns_tl] .
+    move => i E' g' cs lrs .
+    case Henv_tl : (mk_env_ashr_rec E g ls ns_tl (2 * i))
+    => [[[E_tl g_tl] cs_tl] ls_tl] .
+    case Henv_hd : (mk_env_ashr_int E_tl g_tl ls_tl i)
+    => [[[E_hd g_hd] cs_hd] ls_hd] .
+    rewrite /mk_env_ashr_rec -/mk_env_ashr_rec (lock mk_env_ite)
+            /bit_blast_ashr_rec -/bit_blast_ashr_rec (lock bit_blast_ite)
+            /= !theadCons !beheadCons Henv_tl Henv_hd -!lock .
+    case : (ns_hd == lit_tt) .
+    + rewrite (IH _ _ _ _ _ _ _ _ _ Henv_tl) .
+      rewrite (mk_env_ashr_int_is_bit_blast_ashr_int Henv_hd) /= .
+      by case => _ <- <- <- .
+    + case : (ns_hd == lit_ff) .
+      * rewrite (IH _ _ _ _ _ _ _ _ _ Henv_tl) .
+        rewrite (mk_env_ashr_int_is_bit_blast_ashr_int Henv_hd) /= .
+        by case => _ <- <- <- .
+      * rewrite (IH _ _ _ _ _ _ _ _ _ Henv_tl) .
+        rewrite (mk_env_ashr_int_is_bit_blast_ashr_int Henv_hd)
+                (lock mk_env_ite) (lock bit_blast_ite)
+                /= -!lock .
+        case Hite : (mk_env_ite E_hd g_hd ns_hd ls_hd ls_tl)
+        => [[[E_ite g_ite] cs_ite] ls_ite] .
+        rewrite (mk_env_ite_is_bit_blast_ite Hite) .
+        by case => _ <- <- <- .
+Qed .
+
+Lemma mk_env_ashr_is_bit_blast_ashr :
+  forall w E g (ls ns: (w.+1).-tuple literal) E' g' cs lrs,
+    mk_env_ashr E g ls ns = (E', g', cs, lrs) ->
+    bit_blast_ashr g ls ns = (g', cs, lrs).
+Proof.
+  move => w E g ls ns E' g' cs lrs .
+  apply mk_env_ashr_rec_is_bit_blast_ashr_rec .
+Qed .
+
+Lemma mk_env_ashr_int1_newer_gen :
+  forall w E g (ls : (w.+1).-tuple literal) E' g' cs lrs,
+    mk_env_ashr_int1 E g ls = (E', g', cs, lrs) ->
+    (g <=? g')%positive.
+Proof .
+  elim .
+  - move => E g ls E' g' cs lrs .
+    case => _ <- _ _; exact : Pos.leb_refl .
+  - move => n IH E g ls E' g' cs lrs .
+    case => /= _ <- _ _; exact : Pos.leb_refl .
+Qed .
+
+Lemma mk_env_ashr_int_newer_gen :
+  forall w E g (ls : (w.+1).-tuple literal) i E' g' cs lrs,
+    mk_env_ashr_int E g ls i = (E', g', cs, lrs) ->
+    (g <=? g')%positive.
+Proof.
+  move => w E g ls .
+  elim .
+  - move => E' g' cs lrs .
+    case => _ <- _ _ .
+    exact: Pos.leb_refl .
+  - move => n IH E' g' cs lrs .
+    case Henv_tl : (mk_env_ashr_int E g ls n)
+    => [[[E_tl g_tl] cs_tl] lrs_tl] .
+    rewrite /= Henv_tl .
+    case Henv1 : (mk_env_ashr_int1 E_tl g_tl lrs_tl) =>
+    [[[E1 g1] cs1] ls1] .
+    case => _ <- _ _ .
+    exact : (IH _ _ _ _ Henv_tl) .
+Qed .
+
+Lemma mk_env_ashr_rec_newer_gen :
+  forall w wn E g (ls0 : (w.+1).-tuple literal) (ls1 : wn.-tuple literal)
+         i E' g' cs lrs,
+    mk_env_ashr_rec E g ls0 ls1 i = (E', g', cs, lrs) ->
+    (g <=? g')%positive.
+Proof.
+  move => w .
+  elim .
+  - move => E g ls0 ls1 i E' g' cs lrs .
+    case => _ <- _ _ .
+    exact: Pos.leb_refl .
+  - move => n IH E g ls0 /tupleP [ls1_hd ls1_tl] i E' g' cs lrs .
+    case Henv_tl : (mk_env_ashr_rec E g ls0 ls1_tl (2 * i))
+    => [[[E_tl g_tl] cs_tl] lrs_tl] .
+    move : (IH _ _ _ _ _ _ _ _ _ Henv_tl) => Hggtl .
+    rewrite /mk_env_ashr_rec -/mk_env_ashr_rec (lock mk_env_ite)
+            /= !theadCons !beheadCons Henv_tl -lock .
+    case Hshl_int : (mk_env_ashr_int E_tl g_tl lrs_tl i)
+    => [[[E_hd g_hd] cs_hd] ls_hd] .
+    move: (mk_env_ashr_int_newer_gen Hshl_int) => Hgtlghd .
+    case : (ls1_hd == lit_tt) .
+    + case => _ <- _ _ .
+      apply (pos_leb_trans Hggtl Hgtlghd) .
+    + case : (ls1_hd == lit_ff) .
+      * by case => _ <- _ _ .
+      * case Hite : (mk_env_ite E_hd g_hd ls1_hd ls_hd lrs_tl)
+        => [[[E_ite g_ite] cs_ite] ls_ite] .
+        case => _ <- _ _ .
+        move: (mk_env_ite_newer_gen Hite) .
+        move : (pos_leb_trans Hggtl Hgtlghd) .
+        apply pos_leb_trans .
+Qed .
+
+Lemma mk_env_ashr_newer_gen :
+  forall w E g (ls1 ls2 : (w.+1).-tuple literal) E' g' cs lrs,
+    mk_env_ashr E g ls1 ls2 = (E', g', cs, lrs) ->
+    (g <=? g')%positive.
+Proof.
+  move => w E g ls ns E' g' cs lrs .
+  exact : mk_env_ashr_rec_newer_gen .
+Qed .
+
+Lemma mk_env_ashr_int1_newer_res :
+  forall w E g E' g' (ls : (w.+1).-tuple literal) cs lrs,
+    newer_than_lit g lit_tt ->
+    newer_than_lits g ls ->
+    mk_env_ashr_int1 E g ls = (E', g', cs, lrs) ->
+    newer_than_lits g' lrs.
+Proof .
+  elim .
+  - move => E g E' g' ls cs lrs _ Hgls .
+    case => _ <- _ <- /= .
+    by rewrite (newer_than_lits_last _ Hgls) .
+  - move => n IH E g E' g' /tupleP [ls_hd ls_tl] cs lrs Hgtt Hgls .
+    case => _ <- _ <- .
+    rewrite /droplsb /= !beheadCons .
+    move : ls_tl Hgls => /tupleP [ls_tlhd ls_tltl] /= .
+    move => /andP [Hgls_hd] /andP [Hgls_tlhd Hgls_tltl] .
+    apply /andP; split; first by rewrite theadCons .
+    apply newer_than_lits_joinmsb .
+    + apply : (newer_than_lits_default_last Hgls_tltl Hgls_tlhd) .
+    + by rewrite /= .
+Qed .
+
+Lemma mk_env_ashr_int_newer_res :
+  forall w E g i E' g' (ls : (w.+1).-tuple literal) cs lrs,
+    newer_than_lit g lit_tt ->
+    newer_than_lits g ls ->
+    mk_env_ashr_int E g ls i = (E', g', cs, lrs) ->
+    newer_than_lits g' lrs.
+Proof .
+  move => w E g .
+  elim .
+  - move => E' g' ls cs lrs Hgtt Hgls .
+    by case => _ <- _ <- .
+  - move => n IH E' g' ls cs lrs Hgtt Hgls .
+    move Htl : (mk_env_ashr_int E g ls n) => [[[E_tl g_tl] cs_tl] lrs_tl] .
+    rewrite /= Htl .
+    move H1 : (mk_env_ashr_int1 E_tl g_tl lrs_tl) =>
+    [[[E1 g1] cs1] lrs1] .
+    case => _ <- _ <- .
+    move : (IH _ _ _ _ _ Hgtt Hgls Htl) => Hgtllrstl .
+    move : (mk_env_ashr_int_newer_gen Htl) => Hggtl .
+    move : (newer_than_lit_le_newer Hgtt Hggtl) => Hgtltt .
+    rewrite newer_than_lits_joinmsb; first trivial .
+  - move : Hgtltt; rewrite -newer_than_lit_neg /= -/lit_ff => Hgtlff .
+    apply : (newer_than_lits_default_last Hgtllrstl Hgtlff) .
+  - by apply newer_than_lits_behead .
+Qed .
+
+Lemma mk_env_ashr_rec_newer_res :
+  forall w wn E g i E' g'
+         (ls : (w.+1).-tuple literal) (ns : wn.-tuple literal)
+         cs lrs,
+    newer_than_lit g lit_tt ->
+    newer_than_lits g ls -> newer_than_lits g ns ->
+    mk_env_ashr_rec E g ls ns i = (E', g', cs, lrs) ->
+    newer_than_lits g' lrs.
+Proof .
+  move => w .
+  elim .
+  - move => E g i E' g' ls ns cs lrs Hgtt Hgls Hgns .
+    by case => _ <- _ <- .
+  - move => n IH E g i E' g' ls /tupleP [ns_hd ns_tl] cs lrs Hgtt Hgls Hgns .
+    rewrite /mk_env_ashr_rec -/mk_env_ashr_rec (lock mk_env_ite)
+            /= !theadCons !beheadCons -lock .
+    case Henvtl : (mk_env_ashr_rec E g ls ns_tl (2*i))
+    => [[[E_tl g_tl] cs_tl] ls_tl] .
+    case Henvhd : (mk_env_ashr_int E_tl g_tl ls_tl i)
+    => [[[E_hd g_hd] cs_hd] ls_hd] .
+    move : (newer_than_lits_behead Hgns) .
+    rewrite beheadCons => {Hgns} Hgns_tl .
+    move : (IH _ _ _ _ _ _ _ _ _ Hgtt Hgls Hgns_tl Henvtl)
+    => {Hgns_tl} Hgtllstl .
+    case : (ns_hd == lit_tt) .
+    + case => _ <- _ <- .
+      move : (mk_env_ashr_rec_newer_gen Henvtl) => Hggtl .
+      move : (newer_than_lit_le_newer Hgtt Hggtl) => Hgtltt .
+      apply (mk_env_ashr_int_newer_res Hgtltt Hgtllstl Henvhd) .
+    + case : (ns_hd == lit_ff) .
+      * case => _ <- _ <- .
+        done .
+      * case Hite : (mk_env_ite E_hd g_hd ns_hd ls_hd ls_tl)
+        => [[[E_ite g_ite] cs_ite] ls_ite] .
+        case => _ <- _ <- .
+        apply (mk_env_ite_newer_res Hite) .
+Qed .
+
+Lemma mk_env_ashr_newer_res :
+  forall w E g
+         (ls : (w.+1).-tuple literal) (ns : (w.+1).-tuple literal)
+         E' g' cs lrs,
+    newer_than_lit g lit_tt ->
+    newer_than_lits g ls -> newer_than_lits g ns ->
+    mk_env_ashr E g ls ns = (E', g', cs, lrs) ->
+    newer_than_lits g' lrs.
+Proof .
+  move => w E g ls ns E' g' cs lrs .
+  apply mk_env_ashr_rec_newer_res .
+Qed .
+
+Lemma mk_env_ashr_int1_newer_cnf :
+  forall w E g (ls : (w.+1).-tuple literal) E' g' cs lr,
+    mk_env_ashr_int1 E g ls = (E', g', cs, lr) ->
+    newer_than_lits g ls ->
+    newer_than_cnf g' cs.
+Proof .
+  case .
+  - move => E g ls E' g' cs lr .
+    by case => _ <- <- _ _ .
+  - move => n E g ls E' g' cs lr /= .
+    by case => _ <- <- _ .
+Qed .
+
+Lemma mk_env_ashr_int_newer_cnf :
+  forall w E g (ls : (w.+1).-tuple literal) i E' g' cs lr,
+    mk_env_ashr_int E g ls i = (E', g', cs, lr) ->
+    newer_than_lit g lit_tt -> newer_than_lits g ls ->
+    newer_than_cnf g' cs.
+Proof .
+  move => w E g ls .
+  elim .
+  - move => E' g' cs lr .
+    by case => _ <- <- _ _ _ .
+  - move => n IH E' g' cs lr .
+    rewrite /= .
+    case Hn : (mk_env_ashr_int E g ls n) => [[[E_m g_m] cs_m] ls_m] .
+    case H1 : (mk_env_ashr_int1 E_m g_m ls_m) => [[[E1 g1] cs1] ls1] .
+    case => _ <- <- _ Hgtt Hgls .
+    rewrite newer_than_cnf_append .
+    move : (IH _ _ _ _ Hn Hgtt Hgls) => Hgmcsm .
+    move : (mk_env_ashr_int1_newer_gen H1) => Hgmg1 .
+    move : (newer_than_cnf_le_newer Hgmcsm Hgmg1) => {Hgmcsm} Hg1csm .
+    apply /andP; split; last trivial .
+    exact : (IH _ _ _ _ Hn Hgtt Hgls) .
+Qed .
+
+Lemma mk_env_ashr_rec_newer_cnf :
+  forall w wn E g
+         (ls : (w.+1).-tuple literal) (ns : wn.-tuple literal) i
+         E' g' cs lr,
+    mk_env_ashr_rec E g ls ns i = (E', g', cs, lr) ->
+    newer_than_lit g lit_tt ->
+    newer_than_lits g ls -> newer_than_lits g ns ->
+    newer_than_cnf g' cs.
+Proof .
+  move => w .
+  elim .
+  - move => E g ls ns i E' g' cs lr .
+    by case => _ <- <- _ _ _ .
+  - move => n IH E g ls /tupleP [ns_hd ns_tl] i E' g' cs lr .
+    rewrite /mk_env_ashr_rec -/mk_env_ashr_rec (lock mk_env_ite)
+            /= !theadCons !beheadCons -lock .
+    case Htl : (mk_env_ashr_rec E g ls ns_tl (2*i))
+    => [[[E_tl g_tl] cs_tl] ls_tl] .
+    case Hhd : (mk_env_ashr_int E_tl g_tl ls_tl i)
+    => [[[E_hd g_hd] cs_hd] ls_hd] .
+    case : (ns_hd == lit_tt) .
+    + case => _ <- <- _ .
+      move => Hgtt Hgls /andP [Hgnshd Hgnstl] .
+      move : (IH _ _ _ _ _ _ _ _ _ Htl Hgtt Hgls Hgnstl) => Hgtlcstl .
+      move : (mk_env_ashr_rec_newer_res Hgtt Hgls Hgnstl Htl) => Hgtllstl .
+      move : (mk_env_ashr_rec_newer_gen Htl) => Hggtl .
+      move : (newer_than_lit_le_newer Hgtt Hggtl) => Hgtltt .
+      move : (mk_env_ashr_int_newer_cnf Hhd Hgtltt Hgtllstl) => Hghdcshd .
+      move : (mk_env_ashr_int_newer_gen Hhd) => Hgtlghd .
+      move : (newer_than_cnf_le_newer Hgtlcstl Hgtlghd)
+      => Hghdcstl .
+      rewrite newer_than_cnf_append .
+      apply /andP; split; auto .
+    + case : (ns_hd == lit_ff) .
+      * case => _ <- <- _ .
+        move => Hgtt Hgls /andP [Hgnshd Hgnstl] .
+        apply (IH _ _ _ _ _ _ _ _ _ Htl Hgtt Hgls Hgnstl) .
+      * case Hite : (mk_env_ite E_hd g_hd ns_hd ls_hd ls_tl)
+        => [[[E_ite g_ite] cs_ite] ls_ite] .
+        case => _ <- <- _ Hgtt Hgls /andP [Hgnshd Hgnstl] .
+        move : (IH _ _ _ _ _ _ _ _ _ Htl Hgtt Hgls Hgnstl) => Hgtlcstl .
+        move : (mk_env_ashr_rec_newer_res Hgtt Hgls Hgnstl Htl) => Hgtllstl .
+        move : (mk_env_ashr_rec_newer_gen Htl)
+        => { Htl Hgls Hgnstl } Hggtl .
+        move : (newer_than_lit_le_newer Hgtt Hggtl)
+                 (newer_than_lit_le_newer Hgnshd Hggtl)
+        => { Hgtt Hgnshd Hggtl E g } Hgtltt Hgtlnshd .
+        move : (mk_env_ashr_int_newer_cnf Hhd Hgtltt Hgtllstl) => Hghdcshd .
+        move : (mk_env_ashr_int_newer_res Hgtltt Hgtllstl Hhd) => Hghdlshd .
+        move : (mk_env_ashr_int_newer_gen Hhd)
+        => { Hhd Hgtltt } Hgtlghd .
+        move : (newer_than_lit_le_newer Hgtlnshd Hgtlghd)
+                 (newer_than_lits_le_newer Hgtllstl Hgtlghd)
+                 (newer_than_cnf_le_newer Hgtlcstl Hgtlghd)
+        => { Hgtlghd Hgtlnshd Hgtllstl Hgtlcstl E_tl g_tl }
+             Hghdnshd Hghdlstl Hghdcstl .
+        move : (mk_env_ite_newer_cnf Hite Hghdnshd Hghdlshd Hghdlstl)
+        => { Hghdnshd Hghdlshd Hghdlstl } Hgitecsite .
+        move : (mk_env_ite_newer_gen Hite) => Hghdgite .
+        move : (newer_than_cnf_le_newer Hghdcshd Hghdgite)
+                 (newer_than_cnf_le_newer Hghdcstl Hghdgite)
+        => { Hite Hghdcshd Hghdcstl Hghdgite E_hd g_hd }
+             Hgitecshd Hgitecstl .
+        rewrite !newer_than_cnf_append .
+        apply /andP; split; first done .
+        apply /andP; split; done .
+Qed .
+
+Lemma mk_env_ashr_newer_cnf :
+  forall w E g (ls ns : (w.+1).-tuple literal) E' g' cs lrs,
+    mk_env_ashr E g ls ns = (E', g', cs, lrs) ->
+    newer_than_lit g lit_tt ->
+    newer_than_lits g ls -> newer_than_lits g ns ->
+    newer_than_cnf g' cs.
+Proof .
+  rewrite /mk_env_ashr .
+  move => w E g ls ns E' g' cs lrs .
+  exact : mk_env_ashr_rec_newer_cnf .
+Qed .
+
+Lemma mk_env_ashr_int1_preserve :
+  forall w E g (ls : (w.+1).-tuple literal) E' g' cs lrs,
+    mk_env_ashr_int1 E g ls = (E', g', cs, lrs) ->
+    env_preserve E E' g.
+Proof .
+  case .
+  - move => E g ls E' g' cs lrs .
+    by case => <- _ _ _ .
+  - move => n E g ls E' g' cs lrs /= .
+    by case => <- _ _ _ .
+Qed .
+
+Lemma mk_env_ashr_int_preserve :
+  forall w E g (ls : (w.+1).-tuple literal) i E' g' cs lrs,
+    mk_env_ashr_int E g ls i = (E', g', cs, lrs) ->
+    env_preserve E E' g.
+Proof .
+  move => w E g ls .
+  elim .
+  - move => E' g' cs lrs .
+    by case => <- -> _ _ .
+  - move => n IH E' g' cs lrs .
+    case Hn : (mk_env_ashr_int E g ls n) => [[[En gn] csn] lrsn] .
+    move : (IH _ _ _ _ Hn) => HEEn .
+    rewrite /= Hn .
+    move H1 : (mk_env_ashr_int1 En gn lrsn) => [[[E1 g1] cs1] lrs1] .
+    case => <- _ _ _ .
+    move : (mk_env_ashr_int_newer_gen Hn) => Hggn .
+    move : (mk_env_ashr_int1_preserve H1) => HEnE1 .
+    exact : HEEn .
+Qed .
+
+Lemma mk_env_ashr_rec_preserve :
+  forall w wn E g (ls : (w.+1).-tuple literal) (ns : wn.-tuple literal) i
+         E' g' cs lrs,
+    mk_env_ashr_rec E g ls ns i = (E', g', cs, lrs) ->
+    env_preserve E E' g.
+Proof .
+  move => w .
+  elim .
+  - move => E g ls ns i E' g' cs lrs .
+    case => -> _ _ _ .
+    exact : env_preserve_refl .
+  - move => n IH E g ls /tupleP [ns_hd ns_tl] i E' g' cs lrs .
+    rewrite /mk_env_ashr_rec -/mk_env_ashr_rec (lock mk_env_ite)
+            /= !theadCons !beheadCons -lock .
+    case Htl : (mk_env_ashr_rec E g ls ns_tl (2*i))
+    => [[[E_tl g_tl] cs_tl] ls_tl] .
+    move : (IH _ _ _ _ _ _ _ _ _ Htl) => HEEtl .
+    move : (mk_env_ashr_rec_newer_gen Htl) => {Htl} Hggtl .
+    case Hhd : (mk_env_ashr_int E_tl g_tl ls_tl i)
+      => [[[E_hd g_hd] cs_hd] ls_hd] .
+    move : (mk_env_ashr_int_preserve Hhd) => HEtlEhd .
+    move : (env_preserve_le HEtlEhd Hggtl)
+    => { HEtlEhd } HEtlEhd .
+    case : (ns_hd == lit_tt) .
+    + case => <- _ _ _ .
+      by apply (env_preserve_trans HEEtl) .
+    + case : (ns_hd == lit_ff) .
+      * by case => <- .
+      * move : (mk_env_ashr_int_newer_gen Hhd) => Hghdgtl .
+        case Hite : (mk_env_ite E_hd g_hd ns_hd ls_hd ls_tl)
+        => [[[E_ite g_ite] cs_ite] ls_ite] .
+        case => <- _ _ _ .
+        move : (mk_env_ite_preserve Hite) => HEEite .
+        move : (env_preserve_le HEEite Hghdgtl) => {HEEite} HEEite .
+        move : (env_preserve_le HEEite Hggtl) => {HEEite} .
+        apply env_preserve_trans .
+        by apply (env_preserve_trans HEEtl) .
+Qed .
+
+Lemma mk_env_ashr_preserve :
+  forall w E g (ls ns : (w.+1).-tuple literal) E' g' cs lrs,
+    mk_env_ashr E g ls ns = (E', g', cs, lrs) ->
+    env_preserve E E' g.
+Proof .
+  move => w E g ls ns E' g' cs lrs .
+  rewrite /mk_env_ashr. exact : mk_env_ashr_rec_preserve .
+Qed .
+
+Lemma mk_env_ashr_int1_sat :
+  forall w E g (ls : (w.+1).-tuple literal) E' g' cs lrs,
+    mk_env_ashr_int1 E g ls = (E', g', cs, lrs) ->
+    newer_than_lits g ls ->
+    interp_cnf E' cs.
+Proof .
+  case .
+  - move => E g ls E' g' cs lrs .
+    by case => <- _ <- _ _ .
+  - move => n E g ls E' g' cs lrs /= .
+    by case => <- _ <- _ _ .
+Qed .
+
+Lemma mk_env_ashr_int_sat :
+  forall w E g (ls : (w.+1).-tuple literal) i E' g' cs lrs,
+    mk_env_ashr_int E g ls i = (E', g', cs, lrs) ->
+    newer_than_lit g lit_tt -> newer_than_lits g ls ->
+    interp_cnf E' cs.
+Proof .
+  move => w E g ls .
+  elim .
+  - move => E' g' cs lrs .
+    by case => _ _ <- _ _ .
+  - move => n IH E' g' cs lrs .
+    case Hn : (mk_env_ashr_int E g ls n) => [[[En gn] csn] lsn] .
+    rewrite /= Hn .
+    case H1 : (mk_env_ashr_int1 En gn lsn) => [[[E1 g1] cs1] ls1] .
+    case => <- _ <- _ Hgtt Hgls .
+    move : (IH _ _ _ _ Hn Hgtt Hgls) => Hcsn .
+    move : (mk_env_ashr_int_newer_res Hgtt Hgls Hn) => Hgnlsn .
+    move : (mk_env_ashr_int1_sat H1 Hgnlsn) => HE1cs1 .
+    move : (mk_env_ashr_int1_preserve H1) => HEnE1 .
+    move : (mk_env_ashr_int_newer_cnf Hn Hgtt Hgls) => Hgncsn .
+    rewrite -(env_preserve_cnf HEnE1 Hgncsn) in Hcsn .
+    rewrite interp_cnf_append .
+    apply /andP; split; trivial .
+    by rewrite -(env_preserve_cnf HEnE1 Hgncsn) .
+Qed .
+
+Lemma mk_env_ashr_rec_sat :
+  forall w wn E g (ls : (w.+1).-tuple literal) (ns : wn.-tuple literal) i
+         E' g' cs lrs,
+    mk_env_ashr_rec E g ls ns i = (E', g', cs, lrs) ->
+    newer_than_lit g lit_tt -> 
+    newer_than_lits g ls -> newer_than_lits g ns ->
+    interp_cnf E' cs.
+Proof .
+  move => w .
+  elim .
+  - move => E g ls ns i E' g' cs lrs .
+    by case => _ _ <- _ _ _ .
+  - move => n IH E g ls /tupleP [ns_hd ns_tl] i E' g' cs lrs .
+    case Htl : (mk_env_ashr_rec E g ls ns_tl (2 * i))
+    => [[[E_tl g_tl] cs_tl] ls_tl] .
+    case Hhd : (mk_env_ashr_int E_tl g_tl ls_tl i)
+    => [[[E_hd g_hd] cs_hd] ls_hd] .
+    rewrite /mk_env_ashr_rec -/mk_env_ashr_rec (lock mk_env_ite)
+            /= !theadCons !beheadCons Htl Hhd -lock .
+    case : (ns_hd == lit_tt) .
+    + case => <- _ <- _ Hgtt Hgls /andP [Hgnshd Hgnstl] .
+      move : (IH _ _ _ _ _ _ _ _ _ Htl Hgtt Hgls Hgnstl) => HEtlcstl .
+      move : (mk_env_ashr_rec_newer_res Hgtt Hgls Hgnstl Htl) => Hgtllstl .
+      move : (mk_env_ashr_rec_newer_gen Htl) => Hggtl .
+      move : (newer_than_lit_le_newer Hgtt Hggtl) => Hgtltt .
+      move : (mk_env_ashr_int_sat Hhd Hgtltt Hgtllstl) => HEhdcshd .
+      rewrite interp_cnf_append .
+      apply /andP; split; last done .
+      move : (mk_env_ashr_int_preserve Hhd) => HEtlEhd .
+      move : (mk_env_ashr_rec_newer_cnf Htl Hgtt Hgls Hgnstl) => Hgtlcstl .
+      by rewrite (env_preserve_cnf HEtlEhd Hgtlcstl) .
+    + case : (ns_hd == lit_ff) .
+      * case => <- _ <- _ Hgtt Hgls /andP [Hgnshd Hgnstl] .
+        by apply (IH _ _ _ _ _ _ _ _ _ Htl Hgtt Hgls Hgnstl) .
+      * case Hite : (mk_env_ite E_hd g_hd ns_hd ls_hd ls_tl)
+        => [[[E_ite g_ite] cs_ite] ls_ite] .
+        case => <- _ <- _ Hgtt Hgls /andP [Hgnshd Hgnstl] .
+        move : (mk_env_ashr_rec_newer_cnf Htl Hgtt Hgls Hgnstl) => Hgtlcstl .
+        move : (mk_env_ashr_int_preserve Hhd) => HEtlEhd .
+        move : (IH _ _ _ _ _ _ _ _ _ Htl Hgtt Hgls Hgnstl) .
+        rewrite -(env_preserve_cnf HEtlEhd Hgtlcstl)
+        => {HEtlEhd} HEhdcstl .
+        move : (mk_env_ashr_int_newer_gen Hhd) => Hgtlghd .
+        move : (newer_than_cnf_le_newer Hgtlcstl Hgtlghd)
+        => {Hgtlcstl Hgtlghd} Hghdcstl .
+        move : (mk_env_ite_preserve Hite) HEhdcstl => HEhdEite .
+        rewrite -(env_preserve_cnf HEhdEite Hghdcstl) => Hitecstl .
+        move : (mk_env_ashr_rec_newer_res Hgtt Hgls Hgnstl Htl)
+        => {Hgnstl} Hgtllstl .
+        move : (mk_env_ashr_rec_newer_gen Htl) => Hggtl .
+        move : (newer_than_lit_le_newer Hgnshd Hggtl) => Hgtlnshd .
+        move : (newer_than_lit_le_newer Hgtt Hggtl)
+        => { Hgtt Hggtl Hgnshd Htl E } => Hgtltt .
+        move : (mk_env_ashr_int_newer_cnf Hhd Hgtltt Hgtllstl) => Hghdcshd .
+        move : (mk_env_ashr_int_sat Hhd Hgtltt Hgtllstl) .
+        rewrite -(env_preserve_cnf HEhdEite Hghdcshd) => HEitecshd .
+        move : (mk_env_ashr_int_newer_res Hgtltt Hgtllstl Hhd) => Hghdlshd .
+        move : (mk_env_ashr_int_newer_gen Hhd) => Hgtlghd .
+        move : (newer_than_lit_le_newer Hgtlnshd Hgtlghd) => Hghdnshd .
+        move : (newer_than_lits_le_newer Hgtllstl Hgtlghd)
+        => { Hgtlnshd Hgtllstl Hgtlghd } Hghdlstl .
+        move : (mk_env_ite_sat Hite Hghdnshd Hghdlshd Hghdlstl)
+        => { Hghdnshd Hghdlshd Hghdlstl } => HEitecsite .
+        rewrite !interp_cnf_append .
+        apply /andP; split; first done; apply /andP; split; done .
+Qed .
+
+Lemma mk_env_ashr_sat :
+  forall w E g (ls ns : (w.+1).-tuple literal) E' g' cs lrs,
+    mk_env_ashr E g ls ns = (E', g', cs, lrs) ->
+    newer_than_lit g lit_tt -> 
+    newer_than_lits g ls -> newer_than_lits g ns ->
+    interp_cnf E' cs.
+Proof .
+  move => w E g ls ns E' g' cs lrs .
+  rewrite /mk_env_ashr; exact : mk_env_ashr_rec_sat .
+Qed .
 
 
 
@@ -4654,34 +5382,6 @@ Definition bit_blast_signextend w n (g: generator) (ls : (w.+1).-tuple literal) 
 Definition mk_env_signextend w n (E : env) (g : generator) (ls : (w.+1).-tuple literal) : env * generator * cnf * (w.+1 + n).-tuple literal :=
   (E, g, [], cat_tuple ls (nseq_tuple n (last lit_ff ls))) .
 
-Lemma tuple1_behead : forall T (ls : 1.-tuple T), behead ls = [] .
-Proof .
-  move => T .
-  case => [val sz] .
-  apply size0nil .
-  rewrite size_behead /= .
-  by rewrite (eqP sz) .
-Qed .
-
-Lemma enc_bit_last : forall w (bs : BITS w.+1) E ls b l,
-    enc_bits E ls bs ->
-    enc_bit E (last l ls) (last b bs) .
-Proof .
-  elim .
-  - move => bs E ls b l .
-    rewrite enc_bits_splitlsb => /andP [Hencbit _] .
-    rewrite /splitlsb /= in Hencbit .
-    rewrite (tuple_eta ls) (tuple_eta bs) /last /= .
-    by rewrite (tuple1_behead ls) (tuple1_behead bs) .
-  - move => n IH bs E ls b l Hencbit .
-    move: Hencbit; rewrite enc_bits_splitlsb => /andP [_ Hencbits] .
-    rewrite /splitlsb in Hencbits .
-    move: (IH (behead_tuple bs) _ (behead_tuple ls)
-              (thead bs) (thead ls) Hencbits)
-    => {Hencbits} Hencbits .
-    by rewrite (tuple_eta ls) (tuple_eta bs) /last /= .
-Qed .
-
 Lemma bit_blast_signextend_correct :
   forall w n (bs : BITS w.+1) E ls cs,
     enc_bits E ls bs ->
@@ -4690,24 +5390,8 @@ Lemma bit_blast_signextend_correct :
 Proof.
   move => w n bs E ls cs Hlsbs Hprelude .
   rewrite /signExtend /msb /catB /copy .
-  move: (enc_bits_nseq n (enc_bit_last false lit_ff Hlsbs)) => Hlastlsbs .
+  move: (enc_bits_nseq n (enc_bits_last false lit_ff Hlsbs)) => Hlastlsbs .
   exact: (enc_bits_concat Hlastlsbs Hlsbs) .
-Qed .
-
-Lemma newer_than_lits_last :
-  forall w g (ls : (w.+1).-tuple literal) l,
-    newer_than_lits g ls -> newer_than_lit g (last l ls) .
-Proof .
-  elim .
-  - move => g ls l .
-    rewrite (tuple_eta ls) /last /= .
-    rewrite (tuple1_behead ls) .
-    by move /andP => [Hlshd _] .
-  - move => n IH g ls l .
-    rewrite (tuple_eta ls) /= .
-    move /andP => [_ Hlstl] .
-    move: (IH _ (behead_tuple ls) (thead ls) Hlstl) .
-    by rewrite (tuple_eta ls) theadE /= .
 Qed .
 
 
@@ -6896,7 +7580,11 @@ Fixpoint bit_blast_exp w (m : vm) (g : generator) (e : QFBV64.exp w) : vm * gene
     let: (m', g2, cs2, ls2) := bit_blast_exp m1 g1 e2 in
     let: (g', cs, ls) := bit_blast_lshr g2 ls1 ls2 in
     (m', g', cs1 ++ cs2 ++ cs, ls)
-  | QFBV64.bvAshr w e1 e2 => (m, g, [], copy w lit_tt) (* TODO *)
+  | QFBV64.bvAshr w e1 e2 =>
+    let: (m1, g1, cs1, ls1) := bit_blast_exp m g e1 in
+    let: (m', g2, cs2, ls2) := bit_blast_exp m1 g1 e2 in
+    let: (g', cs, ls) := bit_blast_ashr g2 ls1 ls2 in
+    (m', g', cs1 ++ cs2 ++ cs, ls)
   | QFBV64.bvConcat w1 w2 e1 e2 => let '(m1, g1, cs1, rs1) := bit_blast_exp m g e1 in
                                    let '(m', g2, cs2, rs2) := bit_blast_exp m1 g1 e2 in
                                    let '(g', cs, rs) := bit_blast_concat g2 rs1 rs2 in (m', g', cs1 ++ cs2 ++ cs, rs)
@@ -7047,7 +7735,11 @@ Fixpoint mk_env_exp w (m : vm) (s : QFBV64.State.t) (E : env) (g : generator) (e
     let: (m', E2, g2, cs2, ls2) := mk_env_exp m1 s E1 g1 e2 in
     let: (E', g', cs, ls) := mk_env_lshr E2 g2 ls1 ls2 in
     (m', E', g', cs1 ++ cs2 ++ cs, ls)
-  | QFBV64.bvAshr w e1 e2 => (m, E, g, [], copy w lit_tt) (* TODO *)
+  | QFBV64.bvAshr w e1 e2 =>
+    let: (m1, E1, g1, cs1, ls1) := mk_env_exp m s E g e1 in
+    let: (m', E2, g2, cs2, ls2) := mk_env_exp m1 s E1 g1 e2 in
+    let: (E', g', cs, ls) := mk_env_ashr E2 g2 ls1 ls2 in
+    (m', E', g', cs1 ++ cs2 ++ cs, ls)
   | QFBV64.bvConcat w1 w2 e1 e2 =>
     let '(m1, E1, g1, cs1, ls1) := mk_env_exp m s E g e1 in
     let '(m', E2, g2, cs2, ls2) := mk_env_exp m1 s E1 g1 e2 in
@@ -7374,11 +8066,21 @@ Proof.
 Qed .
 
 Lemma bit_blast_exp_preserve_ashr :
-  forall (w0 : nat) (e : QFBV64.exp w0) (e0 : QFBV64.exp w0) (m : vm) (g : generator)
-         (m' : vm) (g' : generator) (cs : cnf) (lrs : w0.-tuple literal),
-    bit_blast_exp m g (QFBV64.bvAshr w0 e e0) = (m', g', cs, lrs) -> vm_preserve m m'.
+  forall (w : nat),
+  forall (e0 : QFBV64.exp (w.+1)),
+      (forall (m : vm) (g : generator) (m' : vm) (g' : generator)
+              (cs : cnf) (lrs : (w.+1).-tuple literal),
+          bit_blast_exp m g e0 = (m', g', cs, lrs) -> vm_preserve m m') ->
+  forall (e1 : QFBV64.exp (w.+1)),
+      (forall (m : vm) (g : generator) (m' : vm) (g' : generator)
+              (cs : cnf) (lrs : (w.+1).-tuple literal),
+          bit_blast_exp m g e1 = (m', g', cs, lrs) -> vm_preserve m m') ->
+    forall (m : vm) (g : generator)
+           (m' : vm) (g' : generator) (cs : cnf) (lrs : (w.+1).-tuple literal),
+      bit_blast_exp m g (QFBV64.bvAshr w e0 e1) = (m', g', cs, lrs) -> vm_preserve m m'.
 Proof.
-Admitted.
+  auto_bit_blast_vm_preserve .
+Qed .
 
 Lemma bit_blast_exp_preserve_concat :
   forall (w0 w1 : nat),
@@ -7781,7 +8483,9 @@ Proof.
   - move=> w e0 e1.
     apply: (bit_blast_exp_preserve_lshr (bit_blast_exp_preserve _ e0)
                                         (bit_blast_exp_preserve _ e1)) .
-  - exact: bit_blast_exp_preserve_ashr.
+  - move=> w e0 e1.
+    apply: (bit_blast_exp_preserve_ashr (bit_blast_exp_preserve _ e0)
+                                        (bit_blast_exp_preserve _ e1)) .
   - move => w0 w1 e0 e1 .
     move: (bit_blast_exp_preserve _ e0) (bit_blast_exp_preserve _ e1)
     => IHe0 IHe1 .
@@ -8250,15 +8954,41 @@ Proof.
 Qed .
 
 Lemma bit_blast_exp_ashr :
-  forall (w0 : nat) (e e0 : QFBV64.exp w0) (m : vm) (g : generator)
-         (s : QFBV64.State.t) (E : env)
-         (m' : vm) (g' : generator) (cs : cnf) (lrs : w0.-tuple literal),
-    bit_blast_exp m g (QFBV64.bvAshr w0 e e0) = (m', g', cs, lrs) ->
-    consistent m' E s ->
-    interp_cnf E (add_prelude cs) ->
-    enc_bits E lrs (QFBV64.eval_exp (QFBV64.bvAshr w0 e e0) s).
+  forall (w : nat),
+    forall (e0 : QFBV64.exp w.+1),
+      (forall (m  : vm) (g  : generator) (s : QFBV64.State.t) (E : env)
+              (m' : vm) (g' : generator)
+              (cs : cnf) (lrs : (w.+1).-tuple literal),
+          bit_blast_exp m g e0 = (m', g', cs, lrs) ->
+          consistent m' E s ->
+          interp_cnf E (add_prelude cs) ->
+          enc_bits E lrs (QFBV64.eval_exp e0 s)) ->
+    forall (e1 : QFBV64.exp w.+1),
+      (forall (m  : vm) (g  : generator) (s : QFBV64.State.t) (E : env)
+              (m' : vm) (g' : generator)
+              (cs : cnf) (lrs : (w.+1).-tuple literal),
+          bit_blast_exp m g e1 = (m', g', cs, lrs) ->
+          consistent m' E s ->
+          interp_cnf E (add_prelude cs) ->
+          enc_bits E lrs (QFBV64.eval_exp e1 s)) ->
+    forall (m : vm) (g : generator) (s : QFBV64.State.t) (E : env)
+           (m' : vm) (g' : generator)
+           (cs : cnf) (lrs : (w.+1).-tuple literal),
+      bit_blast_exp m g (QFBV64.bvAshr w e0 e1) = (m', g', cs, lrs) ->
+      consistent m' E s ->
+      interp_cnf E (add_prelude cs) ->
+      enc_bits E lrs (QFBV64.eval_exp (QFBV64.bvAshr w e0 e1) s).
 Proof.
-Admitted.
+  move => w e0 IHe0 e1 IHe1 m g s E m' g' cs lrs .
+  rewrite (lock interp_cnf) /= -lock. dcase_goal. case; intros; subst.
+  rewrite !add_prelude_append in H7 .
+  move: H7 => /andP [Hcs0 /andP [Hcs1 Hcs2]] .
+  move: (vm_preserve_consistent (bit_blast_exp_preserve H0) H6) => Hcon1.
+  move: (vm_preserve_consistent (bit_blast_exp_preserve H) Hcon1) => Hcon0.
+  move: (IHe0 _ _ _ _ _ _ _ _ H Hcon1 Hcs0) => Hencls0.
+  move: (IHe1 _ _ _ _ _ _ _ _ H0 H6 Hcs1) => Hencls1.
+  apply (bit_blast_ashr_correct H1 Hencls0 Hencls1 Hcs2) .
+Qed .
 
 Lemma bit_blast_exp_concat :
   forall (w0 w1 : nat),
@@ -8955,7 +9685,9 @@ Proof.
   - move => w0 e0 e1 .
     apply: (bit_blast_exp_lshr (bit_blast_exp_correct _ e0)
                                (bit_blast_exp_correct _ e1)) .
-  - exact: bit_blast_exp_ashr.
+  - move => w0 e0 e1 .
+    apply: (bit_blast_exp_ashr (bit_blast_exp_correct _ e0)
+                               (bit_blast_exp_correct _ e1)) .
   - move => w0 w1 e0 e1 .
     move: (bit_blast_exp_correct _ e0) (bit_blast_exp_correct _ e1)
     => IHe0 IHe1 .
@@ -9316,13 +10048,29 @@ Proof.
 Qed .
 
 Lemma mk_env_exp_is_bit_blast_exp_ashr :
-  forall (w0 : nat) (e e0 : QFBV64.exp w0) (m : vm) (E : env)
-         (g : generator) (s : QFBV64.State.t) (m' : vm) (E' : env)
-         (g' : generator) (cs : cnf) (lrs : w0.-tuple literal),
-    mk_env_exp m s E g (QFBV64.bvAshr w0 e e0) = (m', E', g', cs, lrs) ->
-    bit_blast_exp m g (QFBV64.bvAshr w0 e e0) = (m', g', cs, lrs).
+  forall (w : nat),
+    forall (e0 : QFBV64.exp w.+1),
+      (forall (m  : vm) (E  : env) (g  : generator) (s : QFBV64.State.t)
+              (m' : vm) (E' : env) (g' : generator) (cs : cnf)
+              (lrs : (w.+1).-tuple literal),
+          mk_env_exp m s E g e0 = (m', E', g', cs, lrs) ->
+          bit_blast_exp m g e0 = (m', g', cs, lrs)) ->
+    forall (e1 : QFBV64.exp w.+1),
+      (forall (m  : vm) (E  : env) (g  : generator) (s : QFBV64.State.t)
+              (m' : vm) (E' : env) (g' : generator) (cs : cnf)
+              (lrs : (w.+1).-tuple literal),
+          mk_env_exp m s E g e1 = (m', E', g', cs, lrs) ->
+          bit_blast_exp m g e1 = (m', g', cs, lrs)) ->
+    forall (m : vm) (E : env) (g : generator) (s : QFBV64.State.t)
+           (m' : vm) (E' : env) (g' : generator)
+           (cs : cnf) (lrs : (w.+1).-tuple literal),
+      mk_env_exp m s E g (QFBV64.bvAshr w e0 e1) = (m', E', g', cs, lrs) ->
+      bit_blast_exp m g (QFBV64.bvAshr w e0 e1) = (m', g', cs, lrs).
 Proof.
-Admitted.
+  rewrite /=; intros; dcase_hyps; subst.
+  rewrite (H _ _ _ _ _ _ _ _ _ H1) (H0 _ _ _ _ _ _ _ _ _ H3) .
+  by rewrite (mk_env_ashr_is_bit_blast_ashr H2).
+Qed .
 
 Lemma mk_env_exp_is_bit_blast_exp_concat :
   forall (w0 w1 : nat),
@@ -9821,7 +10569,10 @@ Proof.
     apply: (mk_env_exp_is_bit_blast_exp_lshr
               (mk_env_exp_is_bit_blast_exp _ e0)
               (mk_env_exp_is_bit_blast_exp _ e1)) .
-  - exact: mk_env_exp_is_bit_blast_exp_ashr.
+  - move => w e0 e1 .
+    apply: (mk_env_exp_is_bit_blast_exp_ashr
+              (mk_env_exp_is_bit_blast_exp _ e0)
+              (mk_env_exp_is_bit_blast_exp _ e1)) .
   - move => w0 w1 e0 e1 .
     move: (mk_env_exp_is_bit_blast_exp _ e0)
             (mk_env_exp_is_bit_blast_exp _ e1) => IHe0 IHe1 .
@@ -10190,13 +10941,29 @@ Proof.
 Qed .
 
 Lemma mk_env_exp_newer_gen_ashr :
-  forall (w0 : nat) (e e0 : QFBV64.exp w0) (m : vm) (s : QFBV64.State.t)
-         (E : env) (g : generator) (m' : vm) (E' : env) (g' : generator)
-         (cs : cnf) (lrs : w0.-tuple literal),
-    mk_env_exp m s E g (QFBV64.bvAshr w0 e e0) = (m', E', g', cs, lrs) ->
-    (g <=? g')%positive.
+  forall (w : nat),
+    forall (e0 : QFBV64.exp w.+1),
+      (forall (m  : vm) (s  : QFBV64.State.t) (E : env) (g : generator)
+              (m' : vm) (E' : env) (g' : generator) (cs : cnf)
+              (lrs : (w.+1).-tuple literal),
+          mk_env_exp m s E g e0 = (m', E', g', cs, lrs) -> (g <=? g')%positive) ->
+    forall (e1 : QFBV64.exp w.+1),
+      (forall (m  : vm) (s  : QFBV64.State.t) (E : env) (g : generator)
+              (m' : vm) (E' : env) (g' : generator) (cs : cnf)
+              (lrs : (w.+1).-tuple literal),
+          mk_env_exp m s E g e1 = (m', E', g', cs, lrs) -> (g <=? g')%positive) ->
+    forall (m : vm) (s : QFBV64.State.t) (E : env) (g : generator)
+           (m' : vm) (E' : env) (g' : generator)
+           (cs : cnf) (lrs : (w.+1).-tuple literal),
+      mk_env_exp m s E g (QFBV64.bvAshr w e0 e1) = (m', E', g', cs, lrs) ->
+      (g <=? g')%positive.
 Proof.
-Admitted.
+  rewrite /=; intros; dcase_hyps; subst.
+  move: (mk_env_ashr_newer_gen H2) => Hg2g'.
+  move: (H0 _ _ _ _ _ _ _ _ _ H3) => Hg1g2.
+  move: (H  _ _ _ _ _ _ _ _ _ H1) => Hg0g1 .
+  apply: (pos_leb_trans _ Hg2g'). by [ apply: (pos_leb_trans _ Hg1g2)] .
+Qed .
 
 Lemma mk_env_exp_newer_gen_concat :
   forall (w0 w1 : nat),
@@ -10707,7 +11474,9 @@ Proof.
   - move => w e0 e1 .
     exact: (mk_env_exp_newer_gen_lshr
               (mk_env_exp_newer_gen _ e0) (mk_env_exp_newer_gen _ e1)) .
-  - exact: mk_env_exp_newer_gen_ashr.
+  - move => w e0 e1 .
+    exact: (mk_env_exp_newer_gen_ashr
+              (mk_env_exp_newer_gen _ e0) (mk_env_exp_newer_gen _ e1)) .
   - move => w0 w1 e0 e1 .
     move: (mk_env_exp_newer_gen _ e0) (mk_env_exp_newer_gen _ e1)
     => IHe0 IHe1 .
@@ -11090,13 +11859,31 @@ Proof.
 Qed .
 
 Lemma mk_env_exp_newer_vm_ashr :
-  forall (w0 : nat) (e e0 : QFBV64.exp w0) (m : vm) (s : QFBV64.State.t)
-         (E : env) (g : generator) (m' : vm) (E' : env) (g' : generator)
-         (cs : cnf) (lrs : w0.-tuple literal),
-    mk_env_exp m s E g (QFBV64.bvAshr w0 e e0) = (m', E', g', cs, lrs) ->
-    newer_than_vm g m -> newer_than_vm g' m'.
+  forall (w : nat),
+    forall (e0 : QFBV64.exp w.+1),
+      (forall (m : vm) (s : QFBV64.State.t) (E : env) (g : generator)
+              (m' : vm) (E' : env) (g' : generator) (cs : cnf)
+              (lrs : (w.+1).-tuple literal),
+          mk_env_exp m s E g e0 = (m', E', g', cs, lrs) ->
+          newer_than_vm g m -> newer_than_vm g' m') ->
+    forall (e1 : QFBV64.exp w.+1),
+      (forall (m : vm) (s : QFBV64.State.t) (E : env) (g : generator)
+              (m' : vm) (E' : env) (g' : generator) (cs : cnf)
+              (lrs : (w.+1).-tuple literal),
+          mk_env_exp m s E g e1 = (m', E', g', cs, lrs) ->
+          newer_than_vm g m -> newer_than_vm g' m') ->
+    forall (m : vm) (s : QFBV64.State.t) (E : env) (g : generator)
+           (m' : vm) (E' : env) (g' : generator)
+           (cs : cnf) (lrs : (w.+1).-tuple literal),
+      mk_env_exp m s E g (QFBV64.bvAshr w e0 e1) = (m', E', g', cs, lrs) ->
+      newer_than_vm g m -> newer_than_vm g' m'.
 Proof.
-Admitted.
+  rewrite /=; intros; dcase_hyps; subst.
+  move: (mk_env_ashr_newer_gen H3) => Hg2g'.
+  apply: (newer_than_vm_le_newer _ Hg2g').
+  apply: (H0 _ _ _ _ _ _ _ _ _ H4) .
+  by [apply: (H _ _ _ _ _ _ _ _ _ H1)] .
+Qed .
 
 Lemma mk_env_exp_newer_vm_concat :
   forall (w0 w1 : nat),
@@ -11624,7 +12411,9 @@ Proof.
   - move => w e0 e1 .
     exact: (mk_env_exp_newer_vm_lshr (mk_env_exp_newer_vm _ e0)
                                      (mk_env_exp_newer_vm _ e1)) .
-  - exact: mk_env_exp_newer_vm_ashr.
+  - move => w e0 e1 .
+    exact: (mk_env_exp_newer_vm_ashr (mk_env_exp_newer_vm _ e0)
+                                     (mk_env_exp_newer_vm _ e1)) .
   - move => w0 w1 e0 e1 .
     move: (mk_env_exp_newer_vm _ e0) (mk_env_exp_newer_vm _ e1) => IHe0 IHe1 .
     exact: (mk_env_exp_newer_vm_concat IHe0 IHe1) .
@@ -12054,13 +12843,39 @@ Proof.
 Qed .
 
 Lemma mk_env_exp_newer_res_ashr :
-  forall (w0 : nat) (e e0 : QFBV64.exp w0) (m : vm) (s : QFBV64.State.t)
-         (E : env) (g : generator) (m' : vm) (E' : env) (g' : generator)
-         (cs : cnf) (lrs : w0.-tuple literal),
-    mk_env_exp m s E g (QFBV64.bvAshr w0 e e0) = (m', E', g', cs, lrs) ->
-    newer_than_vm g m -> newer_than_lit g lit_tt -> newer_than_lits g' lrs.
+  forall (w : nat),
+    forall (e0 : QFBV64.exp w.+1),
+      (forall (m : vm) (s : QFBV64.State.t) (E : env) (g : generator)
+              (m' : vm) (E' : env) (g' : generator)
+              (cs : cnf) (lrs : (w.+1).-tuple literal),
+          mk_env_exp m s E g e0 = (m', E', g', cs, lrs) ->
+          newer_than_vm g m -> newer_than_lit g lit_tt ->
+          newer_than_lits g' lrs) ->
+    forall (e1 : QFBV64.exp w.+1),
+      (forall (m : vm) (s : QFBV64.State.t) (E : env) (g : generator)
+              (m' : vm) (E' : env) (g' : generator)
+              (cs : cnf) (lrs : (w.+1).-tuple literal),
+          mk_env_exp m s E g e1 = (m', E', g', cs, lrs) ->
+          newer_than_vm g m -> newer_than_lit g lit_tt ->
+          newer_than_lits g' lrs) ->
+    forall (m : vm) (s : QFBV64.State.t) (E : env) (g : generator)
+           (m' : vm) (E' : env) (g' : generator)
+           (cs : cnf) (lrs : (w.+1).-tuple literal),
+      mk_env_exp m s E g (QFBV64.bvAshr w e0 e1) = (m', E', g', cs, lrs) ->
+      newer_than_vm g m -> newer_than_lit g lit_tt -> newer_than_lits g' lrs.
 Proof.
-Admitted.
+  intros w e0 IHe0 e1 IHe1 .
+  rewrite /=; intros; dcase_hyps; subst .
+  move : (mk_env_exp_newer_gen H) => Hgg0 .
+  move : (mk_env_exp_newer_gen H3) => Hg0g1 .
+  move : (mk_env_exp_newer_vm H H0) => Hg0m0 .
+  move : (newer_than_lit_le_newer H1 Hgg0) => {Hgg0} Hg0tt .
+  move : (IHe0 _ _ _ _ _ _ _ _ _ H H0 H1) => {H H0 IHe0} IHg0ls .
+  move : (IHe1 _ _ _ _ _ _ _ _ _ H3 Hg0m0 Hg0tt) => {IHe1 Hg0m0} Hg1ls0 .
+  move : (newer_than_lits_le_newer IHg0ls Hg0g1) => {IHg0ls} Hg1ls .
+  move : (newer_than_lit_le_newer Hg0tt Hg0g1) => {Hg0tt} Hg1tt .
+  exact : (mk_env_ashr_newer_res Hg1tt Hg1ls Hg1ls0 H2) .
+Qed .
 
 Lemma mk_env_exp_newer_res_concat :
   forall (w0 w1 : nat),
@@ -12489,7 +13304,9 @@ Proof.
   - move => w0 e0 e1 .
     exact: (mk_env_exp_newer_res_lshr (mk_env_exp_newer_res _ e0)
                                       (mk_env_exp_newer_res _ e1)) .
-  - exact: mk_env_exp_newer_res_ashr.
+  - move => w0 e0 e1 .
+    exact: (mk_env_exp_newer_res_ashr (mk_env_exp_newer_res _ e0)
+                                      (mk_env_exp_newer_res _ e1)) .
   - move => w0 w1 e0 e1 .
     move: (mk_env_exp_newer_res _ e0) (mk_env_exp_newer_res _ e1)
     => IHe0 IHe1 .
@@ -13032,15 +13849,51 @@ Proof.
 Qed .
 
 Lemma mk_env_exp_newer_cnf_ashr :
-  forall (w0 : nat) (e e0 : QFBV64.exp w0) (m : vm) (s : QFBV64.State.t)
-         (E : env) (g : generator) (m' : vm) (E' : env) (g' : generator)
-         (cs : cnf) (lrs : w0.-tuple literal),
-    mk_env_exp m s E g (QFBV64.bvAshr w0 e e0) = (m', E', g', cs, lrs) ->
-    newer_than_vm g m ->
-    newer_than_lit g lit_tt ->
-    newer_than_cnf g' cs.
+  forall (w : nat),
+    forall (e0 : QFBV64.exp w.+1),
+      (forall (m : vm) (s : QFBV64.State.t) (E : env) (g : generator)
+              (m' : vm) (E' : env) (g' : generator) (cs : cnf)
+              (lrs : (w.+1).-tuple literal),
+          mk_env_exp m s E g e0 = (m', E', g', cs, lrs) ->
+          newer_than_vm g m ->
+          newer_than_lit g lit_tt ->
+          newer_than_cnf g' cs) ->
+    forall (e1 : QFBV64.exp w.+1),
+      (forall (m : vm) (s : QFBV64.State.t) (E : env) (g : generator)
+              (m' : vm) (E' : env) (g' : generator) (cs : cnf)
+              (lrs : (w.+1).-tuple literal),
+          mk_env_exp m s E g e1 = (m', E', g', cs, lrs) ->
+          newer_than_vm g m ->
+          newer_than_lit g lit_tt ->
+          newer_than_cnf g' cs) ->
+    forall (m : vm) (s : QFBV64.State.t) (E : env) (g : generator)
+           (m' : vm) (E' : env) (g' : generator)
+           (cs : cnf) (lrs : (w.+1).-tuple literal),
+      mk_env_exp m s E g (QFBV64.bvAshr w e0 e1) = (m', E', g', cs, lrs) ->
+      newer_than_vm g m ->
+      newer_than_lit g lit_tt ->
+      newer_than_cnf g' cs.
 Proof.
-Admitted.
+  rewrite /=; intros; dcase_hyps; subst. rewrite !newer_than_cnf_append.
+  move: (mk_env_exp_newer_gen H1) => Hgg0 .
+  move: (mk_env_exp_newer_gen H5) => Hg0g1.
+  move: (mk_env_ashr_newer_gen H4) => Hg1g'.
+  (* newer_than_cnf g' cs0 *)
+  move: (H _ _ _ _ _ _ _ _ _ H1 H2 H3) => Hnew_g0cs0.
+  move: (pos_leb_trans Hg0g1 Hg1g') => Hg0g'.
+  rewrite (newer_than_cnf_le_newer Hnew_g0cs0 Hg0g') /=.
+  (* newer_than_cnf g' cs1 *)
+  move: (mk_env_exp_newer_vm H1 H2) => Hnew_g0m0.
+  move: (newer_than_lit_le_newer H3 Hgg0) => {Hgg0} Hg0tt.
+  move: (H0 _ _ _ _ _ _ _ _ _ H5 Hnew_g0m0 Hg0tt) => Hnew_g1cs1.
+  rewrite (newer_than_cnf_le_newer Hnew_g1cs1 Hg1g') /=.
+  (* newer_than_cnf g' cs2 *)
+  move: (mk_env_exp_newer_res H1 H2 H3) => Hnew_g0ls.
+  move: (newer_than_lit_le_newer Hg0tt Hg0g1) => Hg1tt .
+  move: (mk_env_exp_newer_res H5 Hnew_g0m0 Hg0tt) => Hnew_g1ls0 .
+  move: (newer_than_lits_le_newer Hnew_g0ls Hg0g1) => Hnew_g1ls .
+  exact : (mk_env_ashr_newer_cnf H4 Hg1tt Hnew_g1ls Hnew_g1ls0) .
+Qed .
 
 Lemma mk_env_exp_newer_cnf_concat :
   forall (w0 w1 : nat),
@@ -13787,7 +14640,9 @@ Proof.
   - move => w e0 e1 .
     exact: (mk_env_exp_newer_cnf_lshr (mk_env_exp_newer_cnf _ e0)
                                       (mk_env_exp_newer_cnf _ e1)) .
-  - exact: mk_env_exp_newer_cnf_ashr.
+  - move => w e0 e1 .
+    exact: (mk_env_exp_newer_cnf_ashr (mk_env_exp_newer_cnf _ e0)
+                                      (mk_env_exp_newer_cnf _ e1)) .
   - move => w0 w1 e0 e1 .
     move : (mk_env_exp_newer_cnf _ e0) (mk_env_exp_newer_cnf _ e1)
     => IHe0 IHe1 .
@@ -14231,13 +15086,33 @@ Proof.
 Qed .
 
 Lemma mk_env_exp_consistent_ashr :
-  forall (w0 : nat) (e e0 : QFBV64.exp w0) (m : vm) (s : QFBV64.State.t)
-         (E : env) (g : generator) (m' : vm) (E' : env) (g' : generator)
-         (cs : cnf) (lrs : w0.-tuple literal),
-    mk_env_exp m s E g (QFBV64.bvAshr w0 e e0) = (m', E', g', cs, lrs) ->
-    newer_than_vm g m -> consistent m E s -> consistent m' E' s.
+  forall (w : nat),
+    forall (e0 : QFBV64.exp w.+1),
+      (forall (m : vm) (s : QFBV64.State.t) (E : env) (g : generator)
+              (m' : vm) (E' : env) (g' : generator) (cs : cnf)
+              (lrs : (w.+1).-tuple literal),
+          mk_env_exp m s E g e0 = (m', E', g', cs, lrs) ->
+          newer_than_vm g m -> consistent m E s -> consistent m' E' s) ->
+    forall (e1 : QFBV64.exp w.+1),
+      (forall (m : vm) (s : QFBV64.State.t) (E : env) (g : generator)
+              (m' : vm) (E' : env) (g' : generator) (cs : cnf)
+              (lrs : (w.+1).-tuple literal),
+          mk_env_exp m s E g e1 = (m', E', g', cs, lrs) ->
+          newer_than_vm g m -> consistent m E s -> consistent m' E' s) ->
+    forall (m : vm) (s : QFBV64.State.t) (E : env) (g : generator)
+           (m' : vm) (E' : env) (g' : generator)
+           (cs : cnf) (lrs : (w.+1).-tuple literal),
+      mk_env_exp m s E g (QFBV64.bvAshr w e0 e1) = (m', E', g', cs, lrs) ->
+      newer_than_vm g m -> consistent m E s -> consistent m' E' s.
 Proof.
-Admitted.
+  rewrite /=; intros; dcase_hyps; subst.
+  move: (mk_env_exp_newer_vm H1 H2) => Hnew_g0m0.
+  move: (mk_env_exp_newer_vm H5 Hnew_g0m0) => Hnew_g1m'.
+  move: (H _ _ _ _ _ _ _ _ _ H1 H2 H3) => Hm0E0 .
+  move: (mk_env_ashr_preserve H4) => HE1E'g1 .
+  move: (H0 _ _ _ _ _ _ _ _ _ H5 Hnew_g0m0 Hm0E0) => Hm'E1 .
+  exact: (env_preserve_consistent Hnew_g1m' HE1E'g1 Hm'E1) .
+Qed .
 
 Lemma mk_env_exp_consistent_concat :
   forall (w0 w1 : nat),
@@ -14803,7 +15678,9 @@ Proof.
   - move => w e0 e1 .
     exact: (mk_env_exp_consistent_lshr (mk_env_exp_consistent _ e0)
                                        (mk_env_exp_consistent _ e1)) .
-  - exact: mk_env_exp_consistent_ashr.
+  - move => w e0 e1 .
+    exact: (mk_env_exp_consistent_ashr (mk_env_exp_consistent _ e0)
+                                       (mk_env_exp_consistent _ e1)) .
   - move => w0 w1 e0 e1 .
     move: (mk_env_exp_consistent _ e0) (mk_env_exp_consistent _ e1)
     => IHe0 IHe1 .
@@ -15215,13 +16092,36 @@ Proof.
 Qed .
 
 Lemma mk_env_exp_preserve_ashr :
-  forall (w0 : nat) (e e0 : QFBV64.exp w0) (m : vm) (s : QFBV64.State.t)
-         (E : env) (g : generator) (m' : vm) (E' : env) (g' : generator)
-         (cs : cnf) (lrs : w0.-tuple literal),
-    mk_env_exp m s E g (QFBV64.bvAshr w0 e e0) = (m', E', g', cs, lrs) ->
-    env_preserve E E' g.
+  forall (w : nat),
+    forall (e0 : QFBV64.exp w.+1),
+      (forall (m : vm) (s : QFBV64.State.t) (E : env) (g : generator)
+              (m' : vm) (E' : env) (g' : generator) (cs : cnf)
+              (lrs : (w.+1).-tuple literal),
+          mk_env_exp m s E g e0 = (m', E', g', cs, lrs) -> env_preserve E E' g) ->
+    forall (e1 : QFBV64.exp w.+1),
+      (forall (m : vm) (s : QFBV64.State.t) (E : env) (g : generator)
+              (m' : vm) (E' : env) (g' : generator) (cs : cnf)
+              (lrs : (w.+1).-tuple literal),
+          mk_env_exp m s E g e1 = (m', E', g', cs, lrs) -> env_preserve E E' g) ->
+    forall (m : vm) (s : QFBV64.State.t) (E : env) (g : generator)
+           (m' : vm) (E' : env) (g' : generator)
+           (cs : cnf) (lrs : (w.+1).-tuple literal),
+      mk_env_exp m s E g (QFBV64.bvAshr w e0 e1) = (m', E', g', cs, lrs) ->
+      env_preserve E E' g.
 Proof.
-Admitted.
+  rewrite /=; intros; dcase_hyps; subst .
+  move: (H _ _ _ _ _ _ _ _ _ H1) => {H} HEE0g .
+  move: (H0 _ _ _ _ _ _ _ _ _ H3) => {H0} HE0E1g0 .
+  move: (mk_env_exp_newer_gen H1) => Hgg0 .
+  move: (env_preserve_le HE0E1g0 Hgg0) => HE0E1g .
+  move: (env_preserve_trans HEE0g HE0E1g)
+  => {HEE0g HE0E1g0 HE0E1g} HEE1g .
+  move: (mk_env_ashr_preserve H2) => HE1E'g1 .
+  move: (mk_env_exp_newer_gen H3) => Hg0g1 .
+  move: (env_preserve_le HE1E'g1 Hg0g1) => HE1E'g0 .
+  move: (env_preserve_le HE1E'g0 Hgg0) => HE1E'g .
+  exact: (env_preserve_trans HEE1g HE1E'g) .
+Qed .
 
 Lemma mk_env_exp_preserve_concat :
   forall (w0 w1 : nat),
@@ -15762,7 +16662,9 @@ Proof.
   - move => w e0 e1 .
     exact: (mk_env_exp_preserve_lshr (mk_env_exp_preserve _ e0)
                                      (mk_env_exp_preserve _ e1)) .
-  - exact: mk_env_exp_preserve_ashr.
+  - move => w e0 e1 .
+    exact: (mk_env_exp_preserve_ashr (mk_env_exp_preserve _ e0)
+                                     (mk_env_exp_preserve _ e1)) .
   - move => w0 w1 e0 e1 .
     move : (mk_env_exp_preserve _ e0) (mk_env_exp_preserve _ e1)
     => IHe0 IHe1 .
@@ -16415,15 +17317,56 @@ Proof.
 Qed .
 
 Lemma mk_env_exp_sat_ashr :
-  forall (w0 : nat) (e e0 : QFBV64.exp w0) (m : vm) (s : QFBV64.State.t)
-         (E : env) (g : generator) (m' : vm) (E' : env) (g' : generator)
-         (cs : cnf) (lrs : w0.-tuple literal),
-    mk_env_exp m s E g (QFBV64.bvAshr w0 e e0) = (m', E', g', cs, lrs) ->
-    newer_than_vm g m ->
-    newer_than_lit g lit_tt ->
-    interp_cnf E' cs.
+  forall (w : nat),
+    forall (e0 : QFBV64.exp w.+1),
+      (forall (m : vm) (s : QFBV64.State.t) (E : env) (g : generator)
+              (m' : vm) (E' : env) (g' : generator) (cs : cnf)
+              (lrs : (w.+1).-tuple literal),
+          mk_env_exp m s E g e0 = (m', E', g', cs, lrs) ->
+          newer_than_vm g m ->
+          newer_than_lit g lit_tt ->
+          interp_cnf E' cs) ->
+    forall (e1 : QFBV64.exp w.+1),
+      (forall (m : vm) (s : QFBV64.State.t) (E : env) (g : generator)
+              (m' : vm) (E' : env) (g' : generator) (cs : cnf)
+              (lrs : (w.+1).-tuple literal),
+          mk_env_exp m s E g e1 = (m', E', g', cs, lrs) ->
+          newer_than_vm g m ->
+          newer_than_lit g lit_tt ->
+          interp_cnf E' cs) ->
+    forall (m : vm) (s : QFBV64.State.t) (E : env) (g : generator)
+           (m' : vm) (E' : env) (g' : generator)
+           (cs : cnf) (lrs : (w.+1).-tuple literal),
+      mk_env_exp m s E g (QFBV64.bvAshr w e0 e1) = (m', E', g', cs, lrs) ->
+      newer_than_vm g m ->
+      newer_than_lit g lit_tt ->
+      interp_cnf E' cs.
 Proof.
-Admitted.
+  rewrite /=; intros; dcase_hyps; subst. rewrite !interp_cnf_append.
+  move: (mk_env_exp_newer_gen H1) => Hgg0.
+  move: (mk_env_exp_newer_gen H5) => Hg0g1.
+  move: (mk_env_ashr_newer_gen H4) => Hg1g'.
+  move: (mk_env_exp_newer_vm H1 H2) => Hg0m0.
+  move: (mk_env_exp_newer_vm H5 Hg0m0) => Hg1m'.
+  move: (newer_than_lit_le_newer H3 Hgg0) => Hg0tt.
+  move: (newer_than_lit_le_newer Hg0tt Hg0g1) => Hg1tt.
+  move: (mk_env_exp_newer_cnf H1 H2 H3) => Hg0cs0 .
+  move: (mk_env_exp_newer_cnf H5 Hg0m0 Hg0tt) => Hg1cs1 .
+  move: (mk_env_exp_preserve H1) => HEE0g .
+  move: (mk_env_exp_preserve H5) => HE0E1g0 .
+  move: (mk_env_ashr_preserve H4) => HE1E'g1 .
+  (* interp_cnf E' cs0 *)
+  move: (H _ _ _ _ _ _ _ _ _ H1 H2 H3) => HE0cs0 .
+  move: (env_preserve_trans HE0E1g0 (env_preserve_le HE1E'g1 Hg0g1)) => HE0E'g0 .
+  rewrite (env_preserve_cnf HE0E'g0 Hg0cs0) HE0cs0 .
+  (* interp_cnf E' cs1 *)
+  move: (H0 _ _ _ _ _ _ _ _ _ H5 Hg0m0 Hg0tt) => HE1cs1 .
+  rewrite (env_preserve_cnf HE1E'g1 Hg1cs1) HE1cs1 .
+  (* interp_cnf E' cs2 *)
+  move: (newer_than_lits_le_newer (mk_env_exp_newer_res H1 H2 H3) Hg0g1) => Hg1ls .
+  move: (mk_env_exp_newer_res H5 Hg0m0 Hg0tt) => Hg1ls0 .
+  exact: (mk_env_ashr_sat H4 Hg1tt Hg1ls Hg1ls0) => HE2cs2 .
+Qed .
 
 Lemma mk_env_exp_sat_concat :
   forall (w0 w1 : nat),
@@ -17182,7 +18125,8 @@ Proof.
     exact: (mk_env_exp_sat_shl (mk_env_exp_sat _ e0) (mk_env_exp_sat _ e1)) .
   - move => w e0 e1 .
     exact: (mk_env_exp_sat_lshr (mk_env_exp_sat _ e0) (mk_env_exp_sat _ e1)) .
-  - exact: mk_env_exp_sat_ashr.
+  - move => w e0 e1 .
+    exact: (mk_env_exp_sat_ashr (mk_env_exp_sat _ e0) (mk_env_exp_sat _ e1)) .
   - move => w0 w1 e0 e1 .
     move: (mk_env_exp_sat _ e0) (mk_env_exp_sat _ e1) => IHe0 IHe1 .
     exact: (mk_env_exp_sat_concat IHe0 IHe1) .
